examples/Employee_AnalysisModel_UMLPart_generator_deep.thy
@@ -52,7 +52,8 @@ begin
 generation_syntax [ deep
                       (generation_semantics [ analysis (*, oid_start 10*) ])
                       (THEORY Employee_AnalysisModel_UMLPart_generated)
-                      (IMPORTS ["../src/OCL_main", "../src/OCL_class_diagram_static"])
+                      (IMPORTS ["../src/OCL_main", "../src/OCL_class_diagram_static"]
+                               "../src/OCL_class_diagram_generator")
                       SECTION
                       [ in OCaml module_name M (no_signatures) ]
                       (output_directory "../doc") ]
