src/OCL_compiler_aux.thy
@@ -132,6 +132,10 @@ definition "List_split l = (List_map fst l, List_map snd l)"
 definition "List_upto i j = 
  (let to_i = \<lambda>n. int_of_integer (integer_of_natural n) in
   List_map (natural_of_integer o integer_of_int) (upto (to_i i) (to_i j)))"
+definition "List_replace_gen f_res l c0 lby =
+ (case List.fold (\<lambda>c1 (l,lgen). if c1 = c0 then (lby, l # lgen) else (c1 # l, lgen)) (rev l) ([], [])
+  of (l, lgen) \<Rightarrow> f_res (l # lgen))"
+definition "List_replace = List_replace_gen flatten"
 definition "lookup2 rbt = (\<lambda>(x1, x2). Option_bind (\<lambda>rbt. lookup rbt x2) (lookup rbt x1))"
 definition "insert2 = (\<lambda>(x1, x2) v. modify_def empty x1 (insert x2 v))"
 
